Implemented Bitree

Bitree.v
@@ -12,17 +12,19 @@ Inductive tree : Set :=
 Inductive lt_tree : nat -> tree -> Prop :=
   lt_leaf : forall (n   : nat), lt_tree n leaf
 | lt_node : forall (n m : nat) (l r : tree), 
-   m < n -> lt_tree n l -> lt_tree n r -> lt_tree n (node n l r).
+   m < n -> lt_tree n l -> lt_tree n r -> lt_tree n (node m l r).
 
 Inductive gt_tree : nat -> tree -> Prop :=
   gt_leaf : forall (n   : nat), gt_tree n leaf
 | gt_node : forall (n m : nat) (l r : tree), 
-   m > n -> gt_tree n l -> gt_tree n r -> gt_tree n (node n l r).
+   m > n -> gt_tree n l -> gt_tree n r -> gt_tree n (node m l r).
 
 Inductive is_search_tree : tree -> Prop :=
   st_leaf : is_search_tree leaf
 | st_node : forall (n : nat) (l r : tree), 
-   lt_tree n l -> gt_tree n r -> is_search_tree (node n l r).
+   lt_tree n l -> gt_tree n r -> 
+   is_search_tree l -> is_search_tree r -> 
+   is_search_tree (node n l r).
 
 Inductive contains : nat -> tree -> Prop :=
   root_contains : forall (n : nat) (l r : tree), contains n (node n l r)
@@ -33,18 +35,89 @@ Inductive contains : nat -> tree -> Prop :=
 
 Hint Constructors lt_tree gt_tree is_search_tree contains.
 
+Lemma rt_contains: forall (n m : nat), contains m (node n leaf leaf) -> m = n.
+Proof. intros. inversion H; try omega; inversion H2. Qed.
+
+Lemma gt_contains : forall (t : tree) (n : nat), 
+  (forall m, contains m t -> m > n) -> gt_tree n t.
+Proof. intros. induction t; auto. Qed.
+
+Lemma lt_contains : forall (t : tree) (n : nat),
+  (forall m, contains m t -> m < n) -> lt_tree n t.
+Proof. intros. induction t; auto. Qed.
+
+Lemma left_lt : forall (n m : nat) (l r : tree), 
+  is_search_tree (node n l r) -> contains m l -> m < n.
+Proof.
+  intros. induction l. inversion H0. 
+    inversion H. inversion H0. inversion H4. omega.
+      apply IHl1. apply st_node. 
+       inversion H4. assumption. assumption.
+       inversion H6. assumption. assumption. assumption.
+      apply IHl2. apply st_node. 
+       inversion H4. assumption. assumption.
+       inversion H6. assumption. assumption. assumption.
+Qed.
+
+Lemma right_gt : forall (n m : nat) (l r : tree), 
+  is_search_tree (node n l r) -> contains m r -> m > n.
+Proof. 
+  intros. induction r. inversion H0. 
+    inversion H. inversion H0. inversion H5. omega.
+      apply IHr1. apply st_node. assumption.
+       inversion H5. assumption. assumption. 
+       inversion H7. assumption. assumption. 
+      apply IHr2. apply st_node. assumption.
+       inversion H5. assumption. assumption.
+       inversion H7. assumption. assumption.
+Qed.
+
 Definition add_in_search_tree : forall (t : tree) (n : nat),
   is_search_tree t -> 
   {t' | is_search_tree t' & 
-        contains n t' /\ forall (m : nat),
-        contains m t -> contains m t'
+        (forall (m : nat), contains m t' <-> m = n \/ contains m t)
   }.
 Proof.
-  intros. induction t. exists (node n leaf leaf); auto. 
-    assert (L: is_search_tree t1). 
-      
-    remember (lt_eq_lt_dec n n0) as B. inversion B. inversion H0.
-      
+  intros. induction t. 
+    exists (node n leaf leaf). 
+       auto. intros. split. intros. left. 
+       apply rt_contains in H0. assumption. 
+       intros. inversion H0. rewrite H1. auto. inversion H1.    
+    assert (L: is_search_tree t1). inversion H. auto.
+    assert (LT: lt_tree n0 t1). inversion H. auto.
+    assert (R: is_search_tree t2). inversion H. auto.
+    assert (GT: gt_tree n0 t2). inversion H. auto.
+    remember (lt_eq_lt_dec n n0) as B. 
+      inversion B. inversion H0. 
+        apply IHt1 in L. inversion L. 
+          exists (node n0 x t2).
+            apply st_node. apply lt_contains. intros. apply H3 in H4. 
+                inversion H4. omega. apply (left_lt n0 m t1 t2); assumption.
+              assumption. assumption. assumption.
+            intros. split. intros. 
+              inversion H4. right. auto. 
+                apply H3 in H7. inversion H7. left. assumption. right. auto. right. auto.
+            intros. inversion H4. rewrite H5.
+              apply left_contains. apply H3. left. reflexivity.
+              inversion H5. auto. apply left_contains. apply H3. right. assumption.
+                apply right_contains. assumption.
+        exists (node n0 t1 t2). assumption. 
+          intros. split. intros. right. assumption. intros. inversion H2.
+            rewrite <- H1. rewrite H3. auto. assumption.
+        apply IHt2 in R. inversion R.
+          exists (node n0 t1 x).
+            apply st_node. assumption. apply gt_contains. intros. apply H2 in H3.
+                inversion H3. omega. apply (right_gt n0 m t1 t2); assumption.  
+              assumption. assumption.
+            intros. split. intros. 
+              inversion H3. right. auto.
+                right. apply left_contains. assumption. 
+                apply H2 in H6. inversion H6. left. assumption. right. 
+                apply right_contains. assumption.
+            intros. inversion H3. apply right_contains. apply H2. left. assumption.
+                inversion H4. auto. apply left_contains. assumption.
+                apply right_contains. apply H2. right. assumption.
+Qed.
 
 Fixpoint height (t: tree) : nat := 
   match t with
